clarified invariant problem

SpanningTree/SpanningTreeCameras.thy
@@ -19,105 +19,15 @@ type_synonym markingUR = "loc set"
   This would normally be a list of camera functors to allow for modular reasoning.
   Isabelle does not support type lists and thus we use a tuple for this simple example.  
 *)
-type_synonym graphG = "graphUR auth \<times> markingUR auth \<times> heapGS"
+type_synonym graphG = "(graphUR auth \<times> markingUR auth) heapGCmra"
 
 abbreviation own_graph :: "graphUR auth \<Rightarrow> graphG iprop" ("Own\<^sub>g _") where
-  "own_graph \<equiv> \<lambda>g. Own(g, \<epsilon>)"
+  "own_graph \<equiv> \<lambda>g. own_other(g, \<epsilon>)"
 abbreviation own_marking :: "markingUR auth \<Rightarrow> graphG iprop" ("Own\<^sub>m _") where
-  "own_marking \<equiv> \<lambda>m. Own(\<epsilon>, m, \<epsilon>)"
-abbreviation own_heap :: "heapGS \<Rightarrow> graphG iprop" ("Own\<^sub>h _") where
-  "own_heap \<equiv> \<lambda>h. Own(\<epsilon>, \<epsilon>, h)"
+  "own_marking \<equiv> \<lambda>m. own_other(\<epsilon>, m)"
 
-definition points_to_graph :: "loc \<Rightarrow> dfrac \<Rightarrow> val \<Rightarrow> graphG iprop" where
-  "points_to_graph l dq v = Own\<^sub>h(Heap [l\<mapsto>(dq, to_ag (Some v))])"
-abbreviation points_to_disc :: "loc \<Rightarrow> val \<Rightarrow> graphG iprop" where 
-  "points_to_disc \<equiv> \<lambda>l v. points_to_graph l DfracDiscarded v"
-abbreviation points_to_own :: "loc \<Rightarrow> frac \<Rightarrow> val \<Rightarrow> graphG iprop" where
-  "points_to_own \<equiv> \<lambda>l p v. points_to_graph l (DfracOwn p) v"
-abbreviation points_to_full :: "loc \<Rightarrow> val \<Rightarrow> graphG iprop" where
-  "points_to_full \<equiv> \<lambda>l v. points_to_own l 1 v"
 
-bundle graphG_syntax begin
-  notation points_to_graph ("_ \<mapsto>{_} _" 60)
-  notation points_to_disc (infix "\<mapsto>\<box>" 60)
-  notation points_to_own ("_\<mapsto>{#_}_" 60)
-  notation points_to_full (infix "\<mapsto>\<^sub>u" 60)
-end
-
-context includes graphG_syntax begin
-lemma graphG_points_to_valid: "upred_holds ((l \<mapsto>{dq} v) -\<^emph> \<upharpoonleft>(valid dq))"
-proof -
-  have "(l \<mapsto>{dq} v) \<turnstile> \<V>((\<epsilon>, \<epsilon>, Heap [l\<mapsto>(dq,to_ag (Some v))])::graphG)" 
-      by (auto simp: points_to_graph_def own_valid)
-  moreover have "\<V>((\<epsilon>, \<epsilon>, Heap [l\<mapsto>(dq,to_ag (Some v))])::graphG) 
-    \<turnstile> \<upharpoonleft>(valid((\<epsilon>, \<epsilon>, Heap [l\<mapsto>(dq,to_ag (Some v))])::graphG))"
-    using discrete_valid upred_entail_eq_def by auto
-  moreover have "valid((\<epsilon>, \<epsilon>, Heap [l\<mapsto>(dq,to_ag (Some v))])::graphG) 
-    \<longleftrightarrow> valid(Heap [l\<mapsto>(dq,to_ag (Some v))])"
-    by (auto simp: prod_valid_def \<epsilon>_valid)
-  ultimately have "(l \<mapsto>{dq} v) \<turnstile> \<upharpoonleft>(valid dq)" 
-    by (auto simp: frag_heap_valid intro: upred_entails_trans)
-  from upred_wand_holdsI [OF this] show ?thesis .
-qed
-
-lemma graphG_points_to_agree: 
-  "upred_holds ((l \<mapsto>{dq1} v1) -\<^emph> (l \<mapsto>{dq2} v2) -\<^emph> \<upharpoonleft>(v1 = v2))"
-proof -
-  have "upred_holds ((l \<mapsto>{dq1} v1) -\<^emph> (l \<mapsto>{dq2} v2) -\<^emph> 
-    \<V>((\<epsilon>,\<epsilon>,Heap [l\<mapsto>(dq1, to_ag (Some v1))])\<cdot>(\<epsilon>,\<epsilon>,Heap [l\<mapsto>(dq2, to_ag (Some v2))])::graphG))"
-    apply (auto simp: points_to_graph_def) using own_valid2 by auto
-  then have "upred_holds ((l \<mapsto>{dq1} v1) -\<^emph> (l \<mapsto>{dq2} v2) -\<^emph> 
-    \<V>((\<epsilon>,\<epsilon>,Heap ([l\<mapsto>(dq1, to_ag (Some v1))\<cdot>(dq2, to_ag (Some v2))]))::graphG))" 
-    by (auto simp: op_prod_def \<epsilon>_left_id heap_op)
-  from upred_entails_wand_holdsR2[OF upred_entail_eqL[OF discrete_valid] this] 
-  have "upred_holds ((l \<mapsto>{dq1} v1) -\<^emph> (l \<mapsto>{dq2} v2) -\<^emph> 
-    \<upharpoonleft>(All (heap_rel [l\<mapsto>(dq1\<cdot>dq2, to_ag (Some v1)\<cdot>to_ag (Some v2))])))" 
-    by (auto simp: valid_raw_heap.rep_eq valid_def op_prod_def valid_raw_prod_def sprop_conj.rep_eq \<epsilon>_n_valid)
-  then have "upred_holds ((l \<mapsto>{dq1} v1) -\<^emph> (l \<mapsto>{dq2} v2) -\<^emph> 
-    \<upharpoonleft>(valid (dq1\<cdot>dq2) \<and> (\<forall>n. \<exists>ag. n_equiv n (to_ag (Some v1)\<cdot>to_ag (Some v2)) (to_ag ag))))"
-    by (smt (z3) fun_upd_same pure_entailsI upred_entails_wand_holdsR2)
-  then have "upred_holds ((l \<mapsto>{dq1} v1) -\<^emph> (l \<mapsto>{dq2} v2) -\<^emph>
-    \<upharpoonleft>(\<forall>n. \<exists>ag. n_equiv n (to_ag (Some v1)\<cdot>to_ag (Some v2)) (to_ag ag)))"
-    using upred_entails_wand_holdsR2 pure_entailsI by (metis (no_types, lifting))
-  then have "upred_holds ((l \<mapsto>{dq1} v1) -\<^emph> (l \<mapsto>{dq2} v2) -\<^emph> 
-    \<upharpoonleft>(\<exists>ag. to_ag (Some v1)\<cdot>to_ag (Some v2) = to_ag ag))" using d_equiv by (smt (verit, ccfv_SIG))
-  then show ?thesis 
-    by (smt (z3) option.inject pure_entailsI singleton_inject to_ag.rep_eq to_ag_op upred_entails_wand_holdsR2)
-qed
-
-lemma graphG_points_to_combine: 
-  "upred_holds ((l\<mapsto>{dq1} v1) -\<^emph> (l\<mapsto>{dq2} v2) -\<^emph> (l\<mapsto>{dq1\<cdot>dq2} v1) \<^emph> \<upharpoonleft>(v1=v2))"
-  apply (rule upred_wand_holds2I)
-  apply (rule upred_sep_pure)
-  apply (rule entails_pure_extend[OF upred_wandE[OF upred_wand_holdsE[OF graphG_points_to_agree]]])
-  apply (unfold points_to_graph_def)[1]
-  apply (rule upred_entails_trans[OF upred_entail_eqR[OF own_op]])
-  apply (simp add: op_prod_def \<epsilon>_left_id heap_op_val_eq)
-  by (rule upred_wandE[OF upred_wand_holdsE[OF graphG_points_to_agree]])
-
-lemma graphG_points_to_frac_ne: 
-  assumes "\<not> (valid (dq1\<cdot>dq2))"
-  shows "upred_holds ((l1 \<mapsto>{dq1} v1) -\<^emph> (l2 \<mapsto>{dq2} v2) -\<^emph> \<upharpoonleft>(l1\<noteq>l2))"
-proof -
-  from upred_wand_holds2I[OF upred_entails_trans[OF upred_wand_holds2E[OF own_valid2] 
-    upred_entail_eqL[OF discrete_valid]]]
-  have "upred_holds ((l1 \<mapsto>{dq1} v1) -\<^emph> (l2 \<mapsto>{dq2} v2) -\<^emph>
-    \<upharpoonleft>(valid ((\<epsilon>,\<epsilon>,Heap [l1\<mapsto>(dq1,to_ag (Some v1))]) \<cdot> (\<epsilon>,\<epsilon>,Heap [l2\<mapsto>(dq2,to_ag (Some v2))])::graphG)))"
-    by (auto simp: points_to_graph_def)
-  then have base: "upred_holds ((l1 \<mapsto>{dq1} v1) -\<^emph> (l2 \<mapsto>{dq2} v2) -\<^emph>
-    \<upharpoonleft>(valid ((Heap [l1\<mapsto>(dq1,to_ag (Some v1))]) \<cdot> (Heap [l2\<mapsto>(dq2,to_ag (Some v2))]))))"
-    by (auto simp: op_prod_def \<epsilon>_left_id prod_valid_def \<epsilon>_valid)
-  from assms have "\<not> (\<forall>n. heap_rel ([l1\<mapsto>(dq1,to_ag (Some v1))\<cdot>(dq2,to_ag (Some v2))]) n)"
-    by (auto simp: op_fun_def valid_def op_prod_def)
-  with heap_valid_op have "valid ((Heap [l1\<mapsto>(dq1,to_ag (Some v1))]) \<cdot> (Heap [l2\<mapsto>(dq2,to_ag (Some v2))])) =
-    (l1\<noteq>l2 \<and> valid (Heap [l1\<mapsto>(dq1,to_ag (Some v1))]) \<and> valid (Heap [l2\<mapsto>(dq2,to_ag (Some v2))]))"
-    by metis
-  then have "\<upharpoonleft>(valid ((Heap [l1\<mapsto>(dq1,to_ag (Some v1))]) \<cdot> (Heap [l2\<mapsto>(dq2,to_ag (Some v2))]))) \<turnstile>
-    \<upharpoonleft>(l1\<noteq>l2)" using pure_entailsI by blast
-  from upred_entails_wand_holdsR2[OF this base] show ?thesis .
-qed
-
-lemma graphG_points_to_ne: "upred_holds ((l1\<mapsto>\<^sub>uv1) -\<^emph> (l2\<mapsto>{dq2} v2) -\<^emph> \<upharpoonleft>(l1\<noteq>l2))"
-  by (rule graphG_points_to_frac_ne[OF dfrac_not_valid_own])
+context includes points_to_syntax begin
+lemma  "upred_holds (((l \<mapsto>{dq} v)::graphG iprop) -\<^emph> \<upharpoonleft>(valid dq))" by (rule points_to_valid)
 end
 end
