HeapLang/WeakestPrecondition.thy
@@ -5,31 +5,29 @@ begin
 subsection \<open>Weakest Preconditions\<close>
 text \<open>
   The functions below mirror the stepwise derivation of wp from "Iris from ground up".
-  wp2 and wp3 differ to the paper description in that they take a \<Phi> which does not return iprop 
-  but only the underlying camera. This needs to be changed lateron but helps typechecking for now.
 \<close>
 function wp1 :: "expr \<Rightarrow> (val \<Rightarrow> ('a::ucamera) iprop) \<Rightarrow> 'a iprop" where
   "wp1 e \<Phi> = (case to_val e of Some v \<Rightarrow> \<Phi> v 
-    | None \<Rightarrow> \<forall>\<^sub>u(\<lambda>\<sigma>. (\<upharpoonleft>(red e \<sigma>)) \<and>\<^sub>u \<triangleright>(\<forall>\<^sub>u(\<lambda>(\<kappa>,e2,\<sigma>2). (\<upharpoonleft>(e \<sigma> \<kappa> \<Rightarrow>\<^sub>h e2 \<sigma>2 [])) -\<^emph> wp1 e2 \<Phi>))))"
+    | None \<Rightarrow> (\<forall>\<^sub>u \<sigma>. ((\<upharpoonleft>(red e \<sigma>)) \<and>\<^sub>u \<triangleright>(\<forall>\<^sub>u \<kappa> e2 \<sigma>2. (\<upharpoonleft>(e \<sigma> \<kappa> \<Rightarrow>\<^sub>h e2 \<sigma>2 [])) -\<^emph> wp1 e2 \<Phi>))))"
     by fastforce blast
 
-definition own_state_heap :: "state \<Rightarrow> (loc,val option,'c::ucamera) heapCmra iprop" where
+definition own_state_heap :: "state \<Rightarrow> 'a::ucamera heapGCmra iprop" where
   "own_state_heap s = Own\<^sub>h (full (to_heap_op (heap s)))"
 
-function wp2 :: "expr \<Rightarrow> (val \<Rightarrow> 'a::ucamera) \<Rightarrow> (loc,val option,'a) heapCmra iprop" where
-  "wp2 e \<Phi> = (case to_val e of Some v \<Rightarrow> \<Rrightarrow>\<^sub>b (own_other (\<Phi> v))
-    | None \<Rightarrow> \<forall>\<^sub>u(\<lambda>\<sigma>. own_state_heap \<sigma> -\<^emph>
-      \<Rrightarrow>\<^sub>b ((\<upharpoonleft>(red e \<sigma>)) \<and>\<^sub>u \<triangleright>(\<forall>\<^sub>u(\<lambda>(\<kappa>,e2,\<sigma>2). (\<upharpoonleft>(e \<sigma> \<kappa> \<Rightarrow>\<^sub>h e2 \<sigma>2 [])) -\<^emph> 
+function wp2 :: "expr \<Rightarrow> (val \<Rightarrow> 'a::ucamera heapGCmra iprop) \<Rightarrow> 'a heapGCmra iprop" where
+  "wp2 e \<Phi> = (case to_val e of Some v \<Rightarrow> \<Rrightarrow>\<^sub>b (\<Phi> v)
+    | None \<Rightarrow> (\<forall>\<^sub>u \<sigma>. (own_state_heap \<sigma> -\<^emph>
+      \<Rrightarrow>\<^sub>b ((\<upharpoonleft>(red e \<sigma>)) \<and>\<^sub>u \<triangleright>(\<forall>\<^sub>u \<kappa> e2 \<sigma>2. (\<upharpoonleft>(e \<sigma> \<kappa> \<Rightarrow>\<^sub>h e2 \<sigma>2 [])) -\<^emph> 
         \<Rrightarrow>\<^sub>b ((own_state_heap \<sigma>2) \<^emph> wp2 e2 \<Phi>))))))"
    by fast simp
 
-function wp3 :: "expr \<Rightarrow> (val \<Rightarrow> 'a::ucamera) \<Rightarrow> (loc,val option,'a) heapCmra iprop" where
-  "wp3 e \<Phi> = (case to_val e of Some v \<Rightarrow> \<Rrightarrow>\<^sub>b (own_other (\<Phi> v))
-    | None \<Rightarrow> \<forall>\<^sub>u(\<lambda>\<sigma>. own_state_heap \<sigma> -\<^emph>
-      \<Rrightarrow>\<^sub>b ((\<upharpoonleft>(red e \<sigma>)) \<and>\<^sub>u \<triangleright>(\<forall>\<^sub>u(\<lambda>(\<kappa>,e2,\<sigma>2,efs). (\<upharpoonleft>(e \<sigma> \<kappa> \<Rightarrow>\<^sub>h e2 \<sigma>2 efs)) -\<^emph> 
-        \<Rrightarrow>\<^sub>b ((own_state_heap \<sigma>2) \<^emph> wp3 e2 \<Phi> \<^emph> (sep_map_set (\<lambda>e'. wp3 e' (\<lambda>_. \<epsilon>)) (set efs))))))))"
+function wp3 :: "expr \<Rightarrow> (val \<Rightarrow> 'a::ucamera heapGCmra iprop) \<Rightarrow> 'a heapGCmra iprop" where
+  "wp3 e \<Phi> = (case to_val e of Some v \<Rightarrow> \<Rrightarrow>\<^sub>b (\<Phi> v)
+    | None \<Rightarrow> (\<forall>\<^sub>u \<sigma>. (own_state_heap \<sigma> -\<^emph>
+      \<Rrightarrow>\<^sub>b ((\<upharpoonleft>(red e \<sigma>)) \<and>\<^sub>u \<triangleright>(\<forall>\<^sub>u \<kappa> e2 \<sigma>2 efs. (\<upharpoonleft>(e \<sigma> \<kappa> \<Rightarrow>\<^sub>h e2 \<sigma>2 efs)) -\<^emph> 
+        \<Rrightarrow>\<^sub>b ((own_state_heap \<sigma>2) \<^emph> wp3 e2 \<Phi> \<^emph> (sep_map_set (\<lambda>e'. wp3 e' (\<lambda>_. \<upharpoonleft>True)) (set efs))))))))"
   by fast auto
 
-abbreviation wp :: "expr \<Rightarrow> (val \<Rightarrow> 'a::ucamera) \<Rightarrow> (loc,val option,'a) heapCmra iprop" where 
+abbreviation wp :: "expr \<Rightarrow> (val \<Rightarrow> 'a::ucamera heapGCmra iprop) \<Rightarrow> 'a heapGCmra iprop" where 
   "wp \<equiv> wp3"
 end
